src/LiftedComp.v
@@ -3,6 +3,8 @@ Require Import Monads.
 Require Import ListLemmas.
 Require Import Metadata.
 
+
+
 Require Untyped.
 Require Lifted.
 Require Utopia.
@@ -143,33 +145,40 @@ Definition compile_cu (cu : list U.expr * list metadata) : list L.expr * list me
   
 End compile.
 
+Require Import CompilationUnit.
+Require Import Semantics.
 
 Section Simulation.
 
-
   Variable prog : list U.expr * list metadata.
+  Variable prog' : list U.expr * list metadata.
   Variable tprog : list L.expr * list metadata.
-  Hypothesis TRANSF : compile_cu prog = tprog.
-  
-  Inductive match_states : L.env -> U.expr -> L.expr -> Prop :=.
+  Hypothesis MD_INIT : Metadata.check_length prog = Some prog'.
+  Hypothesis TRANSF : compile_cu prog' = tprog.
 
-  Lemma step_sim :
-    forall el el' er E,
-      match_states E el er ->
-      U.step el el' ->
-      exists er',
-        L.step E er er' /\ match_states E el' er'.
+  Theorem fsim :
+    forward_simulation (Untyped.semantics prog) (Lifted.semantics tprog).
   Proof.
   Admitted.
+  (* Inductive match_states : L.env -> U.expr -> L.expr -> Prop :=. *)
 
-  Lemma initial_state_exists :
-      forall expr,
-        U.initial_state prog expr ->
-        exists expr' E,
-          L.initial_state tprog expr' /\
-          match_states E expr expr'.
-  Proof.
-  Admitted.
+  (* Lemma step_sim : *)
+  (*   forall el el' er E, *)
+  (*     match_states E el er -> *)
+  (*     U.step el el' -> *)
+  (*     exists er', *)
+  (*       L.step E er er' /\ match_states E el' er'. *)
+  (* Proof. *)
+  (* Admitted. *)
+
+  (* Lemma initial_state_exists : *)
+  (*     forall expr, *)
+  (*       U.initial_state prog expr -> *)
+  (*       exists expr' E, *)
+  (*         L.initial_state tprog expr' /\ *)
+  (*         match_states E expr expr'. *)
+  (* Proof. *)
+  (* Admitted. *)
 
   
 End Simulation.
